### Derivations ###

Orbital Velocity:

Setting Gravitational force = Centripetal force

$F_g$ = $\frac{G M m}{r^2}$

where: 
G => gravitational constant 
M => mass of the larger object about which the smaller object orbits
m => mass of the orbiting body 
r => distance between the two objects.

Centripetal force is defined as mass times acceleration, where we are considering centripetal acceleration 
a
c
:

⇒
F
c
=
m
a
c
=
m
v
2
r
 

where 
m
 is the mass of the object undergoing uniform circular motion, 
v
 is its speed, and 
r
 is the radius of the circle defined by its motion.

Now we equate:

⇒
F
g
=
F
c

⇒
G
M
m
r
2
=
m
v
2
r

We want to find 
v
:

⇒
G
M
m
r
2
=
m
v
2
r

⇒
G
M
r
=
v
2

Hence:

⇒
v
=
±
√
G
M
r

If you're only concerned with magnitude, just take the positive result:

⇒
v
=
√
G
M
r

